

MAT2LG

Assignment 2

Name: Mazidul Blam Kabbo

ID: 24301500

Section: 17

$$1 \quad A = \begin{bmatrix} -2 & 0 & 0 & 0 \\ 0 & -2 & 0 & 0 \\ 0 & 0 & 5 & 0 \\ 0 & 0 & 0 & 3 \end{bmatrix}$$

we know, $|A - \lambda I| = 0$, so $Ax = \lambda x$, where x is an eigenvector corresp to λ , where scalar λ is an eigenvalue

$$\begin{aligned} |A - \lambda I| &= \begin{vmatrix} -2-\lambda & 0 & 0 & 0 \\ 0 & -2-\lambda & 0 & 0 \\ 0 & 0 & 5-\lambda & 0 \\ 0 & 0 & 0 & 3-\lambda \end{vmatrix} = \begin{vmatrix} -2-\lambda & 0 & 0 & 0 \\ 0 & -2-\lambda & 0 & 0 \\ 0 & 0 & 5-\lambda & 0 \\ 0 & 0 & 0 & 3-\lambda \end{vmatrix} \\ &= (-2-\lambda) \begin{vmatrix} -2-\lambda & 0 & 0 \\ 0 & 5-\lambda & 0 \\ 0 & 0 & 3-\lambda \end{vmatrix} \\ &= (-2-\lambda)(-2-\lambda) \begin{vmatrix} 5-\lambda & 0 \\ 0 & 3-\lambda \end{vmatrix} \\ &= (-2-\lambda)(-2-\lambda)(5-\lambda)(3-\lambda) = 0 \end{aligned}$$

$$\lambda = -2, 3, -2, 3$$

For $\lambda = -2$

$$A - \lambda I = \begin{bmatrix} 0 & 0 & 0 & 0 \\ 0 & 0 & 0 & 0 \\ 0 & 0 & 5 & 0 \\ 0 & 0 & 0 & 5 \end{bmatrix} \quad R_2' = R_2 - R_3 + R_4$$

$$\begin{bmatrix} 0 & 0 & 0 & 0 \\ 0 & 0 & 0 & 0 \\ 0 & 0 & 5 & 0 \\ 0 & 0 & 0 & 5 \end{bmatrix} \Rightarrow \begin{cases} 0x_1 + 0x_2 + 0x_3 + 0x_4 = 0 \\ 0x_1 + 0x_2 + 0x_3 + 0x_4 = 0 \\ 0x_1 + 0x_2 + 5x_3 + 0x_4 = 0 \\ 0x_1 + 0x_2 + 0x_3 + 5x_4 = 0 \end{cases}$$

$$5x_3 = 0$$

$$x_3 = 0$$

$$5x_4 = 0$$

$$x_4 = 0$$

$$\text{let } x_1 = s, x_2 = t, \text{ so}$$

$$\begin{pmatrix} x_1 \\ x_2 \\ x_3 \\ x_4 \end{pmatrix} = \begin{pmatrix} s \\ t \\ 0 \\ 0 \end{pmatrix}$$

$$s \begin{pmatrix} 1 \\ 0 \\ 0 \\ 0 \end{pmatrix} + t \begin{pmatrix} 0 \\ 1 \\ 0 \\ 0 \end{pmatrix}$$

eigenvectors with respect to $\lambda = -2$

$$E_{-2} = \text{Span} \left\{ \begin{pmatrix} 1 \\ 0 \\ 0 \\ 0 \end{pmatrix}, \begin{pmatrix} 0 \\ 1 \\ 0 \\ 0 \end{pmatrix} \right\}$$

For $\lambda = 3$

$$A - \lambda I = \begin{bmatrix} -5 & 0 & 0 & 0 \\ 0 & -5 & 0 & 0 \\ 0 & 0 & 0 & 0 \\ 0 & 0 & 0 & 0 \end{bmatrix} \Rightarrow \begin{cases} -5x_1 + 0x_2 + 0x_3 + 0x_4 = 0 \\ 0x_1 - 5x_2 + 0x_3 - 0x_4 = 0 \\ 0x_1 + 0x_2 + 0x_3 + 0x_4 = 0 \\ 0x_1 + 0x_2 + 0x_3 + 0x_4 = 0 \end{cases}$$

$$-5x_1 = 0$$

$$x_1 = 0$$

$$\text{let } x_3 = s, x_4 = t$$

$$-5x_2 + 5x_3 - 5x_4 = 0$$

$$-5x_2 + 5s - 5t = 0$$

$$x_2 = s - t$$

$$\begin{pmatrix} x_1 \\ x_2 \\ x_3 \\ x_4 \end{pmatrix} = \begin{pmatrix} 0 \\ s-t \\ s \\ t \end{pmatrix}$$

eigenvector with respect to $\lambda = 3$

$$E_3 = \text{Span} \left\{ \begin{pmatrix} 0 \\ 1 \\ 1 \\ 0 \end{pmatrix}, \begin{pmatrix} 0 \\ -1 \\ 0 \\ 1 \end{pmatrix} \right\}$$

$$P = \begin{bmatrix} 1 & 0 & 0 & 0 \\ 0 & 1 & 0 & 0 \\ 0 & 0 & 1 & 0 \\ 0 & 0 & 0 & 1 \end{bmatrix}$$

$$P^{-1}AP = \begin{bmatrix} 2 & 0 & 0 & 0 \\ 0 & -2 & 0 & 0 \\ 0 & 0 & 3 & 0 \\ 0 & 0 & 0 & 3 \end{bmatrix}$$

2. $f(x) = x \sin x, -\pi < x < \pi \Rightarrow 2L = 2\pi \Rightarrow L = \pi$

For Fourier series,

$$f(x) = \frac{a_0}{2} + \sum_{n=1}^{\infty} a_n \cos nx + \sum_{n=1}^{\infty} b_n \sin nx$$

$$a_n = \frac{1}{\pi} \int_{-\pi}^{\pi} x \sin x \cos nx \, dx$$

we know

$$\begin{aligned} \Rightarrow \quad u &= x \\ du &= 1 \\ dv &= \sin x \cos nx \\ v &= \int \sin x \cos nx \, dx \\ &= \frac{1}{2} \int \sin(x+nx) + \sin(x-nx) \, dx \\ &= \frac{1}{2} \int \sin(1+n)x + \sin(1-n)x \, dx \\ &= \frac{1}{2} \left[\frac{-\cos(1+n)x}{1+n} - \frac{\cos(1-n)x}{1-n} \right] \end{aligned}$$

$$\sin A \cos B = \frac{1}{2} (\sin(A+B) + \sin(A-B))$$

$A = x$
 $B = nx$

$$\begin{aligned} a_n &= \frac{1}{\pi} \left[\frac{x}{2} \left(\frac{-\cos(1+n)x}{1+n} - \frac{\cos(1-n)x}{1-n} \right) - \frac{1}{2} \int \frac{-\cos(1+n)x}{1+n} - \frac{\cos(1-n)x}{1-n} \, dx \right]_{-\pi}^{\pi} \\ &= \frac{1}{\pi} \left[\frac{x}{2} \left(\frac{-\cos(1+n)x}{1+n} - \frac{\cos(1-n)x}{1-n} \right) + \frac{1}{2} \left(\frac{\sin(1+n)x}{(1+n)^2} + \frac{\sin(1-n)x}{(1-n)^2} \right) \right]_{-\pi}^{\pi} \\ &= \frac{1}{\pi} \left(\frac{\pi}{2} \left(\frac{-\cos(1+n)\pi}{1+n} - \frac{\cos(1-n)\pi}{1-n} \right) + \frac{1}{2} \frac{\sin(1+n)\pi}{(1+n)^2} + \frac{1}{2} \frac{\sin(1-n)\pi}{(1-n)^2} \right. \\ &\quad \left. - \frac{\pi}{2} \left(\frac{-\cos(1+n)(-\pi)}{1+n} - \frac{\cos(1-n)(-\pi)}{1-n} \right) - \frac{1}{2} \frac{\sin(1+n)\pi}{(1+n)^2} - \frac{1}{2} \frac{\sin(1-n)\pi}{(1-n)^2} \right) \end{aligned}$$

we know, $\sin k\pi = 0, \cos A = \cos(-A)$

$$\begin{aligned} \text{So,} \quad & \frac{1}{\pi} \left(\frac{\pi}{2} \left(\frac{-\cos(1+n)\pi}{1+n} - \frac{\cos(1-n)\pi}{1-n} \right) + \frac{1}{2} \left(\frac{-\cos(1+n)\pi}{1+n} - \frac{\cos(1-n)\pi}{1-n} \right) \right) \\ &= -\frac{1}{2} \frac{\cos(1+n)\pi}{1+n} - \frac{1}{2} \frac{\cos(1-n)\pi}{1-n} - \frac{1}{2} \frac{\cos(1+n)\pi}{1+n} - \frac{1}{2} \frac{\cos(1-n)\pi}{1-n} \\ &= -\frac{\cos \pi + n\pi}{1+n} - \frac{\cos \pi - n\pi}{1-n} \quad [\cos(A+B) = \cos A \cos B - \sin A \sin B] \\ &= -\frac{\cos \pi \cos n\pi - \sin \pi \sin n\pi}{n+1} - \frac{\cos \pi \cos n\pi - \sin \pi \sin n\pi}{1-n} \end{aligned}$$

$$\frac{\cos n\pi}{1+n} + \frac{\cos n\pi}{1-n}$$

$$\frac{(-1)^n (1+n+1-n)}{1-n^2}$$

$$\frac{2(-1)^n}{1-n^2} = a_n$$

$$\begin{aligned} a_0 &= \frac{2(-1)^0}{1-0^2} \\ &= 2 \end{aligned}$$

$$b_n = \frac{1}{\pi} \int_{-\pi}^{\pi} x \sin x \sin nx \, dx$$

\Rightarrow

$$\begin{aligned} u &= x \\ du &= 1 \\ dv &= \sin x \sin nx \\ v &= \int \sin x \sin nx \, dx \end{aligned}$$

we know,

$$\cos(A+B) = \cos A \cos B - \sin A \sin B$$

$$\cos(A-B) = \cos A \cos B + \sin A \sin B$$

$$\cos(A-B) - \cos(A+B) = 2 \sin A \sin B$$

$$\frac{1}{2} \cos(A-B) - \frac{1}{2} \cos(A+B) = \sin A \sin B$$

$$A=x, B=nx$$

$$b_n = \frac{1}{\pi} \left[\frac{x}{2} \left(\frac{\sin(1-n)x}{1-n} - \frac{\sin(1+n)x}{1+n} \right) - \frac{1}{2} \int \frac{\sin(1-n)x}{1-n} - \frac{\sin(1+n)x}{1+n} \right]_{-\pi}^{\pi}$$

$$= \frac{1}{\pi} \left[\frac{x}{2} \left(\frac{\sin(1-n)x}{1-n} - \frac{\sin(1+n)x}{1+n} \right) + \frac{1}{2} \frac{\cos(1-n)x}{(1-n)^2} - \frac{1}{2} \frac{\cos(1+n)x}{(1+n)^2} \right]_{-\pi}^{\pi}$$

$$= \frac{1}{\pi} \left(\frac{\pi}{2} \frac{\cos(1-n)\pi}{(1-n)^2} - \frac{\pi}{2} \frac{\cos(1+n)\pi}{(1+n)^2} - \frac{1}{2} \frac{\cos(1-n)\pi}{(1-n)^2} + \frac{1}{2} \frac{\cos(1+n)\pi}{(1+n)^2} \right)$$

$$\text{we know, } \cos(A) = \cos(-A)$$

$$= \left(\frac{1}{2} \frac{\cos(1-n)\pi}{(1-n)^2} - \frac{1}{2} \frac{\cos(1-n)\pi}{(1-n)^2} - \frac{1}{2} \frac{\cos(1+n)\pi}{(1+n)^2} + \frac{1}{2} \frac{\cos(1+n)\pi}{(1+n)^2} \right)$$

$$b_n = 0$$

$$f(x) = 1 + \sum_{n=1}^{\infty} \frac{2(-1)^n}{1-n^2} \cos nx \quad (\text{Ans})$$

$$3. \quad f(x) = \begin{cases} x & 0 < x < 4 \\ 8-x & 4 < x < 8 \end{cases} \quad L=8$$

$$\begin{aligned} a_0 &= 0 \\ a_n &= 0 \end{aligned}$$

$$f(x) = \sum_{n=1}^{\infty} b_n \sin \frac{n\pi x}{L}$$

$$b_n = \frac{2}{L} \int_0^4 x \sin \frac{n\pi x}{8} \, dx + \frac{2}{L} \int_4^8 (8-x) \sin \frac{n\pi x}{8} \, dx$$

$$\frac{2}{8} \int_0^4 x \sin \frac{n\pi x}{8} \, dx$$

$$= \frac{1}{4} \left[x \left(-\frac{8}{n\pi} \cos \frac{n\pi x}{8} \right) + \frac{8}{n\pi} \int \cos \frac{n\pi x}{8} \, dx \right]_0^4$$

$$= \frac{1}{4} \left[x \left(-\frac{8}{n\pi} \cos \frac{n\pi x}{8} \right) + \frac{64}{n^2\pi} \sin \frac{n\pi x}{8} \right]_0^4$$

$$= \frac{1}{4} \left(-\frac{32}{n\pi} \cos \frac{1}{2} n\pi + \frac{64}{n^2\pi} \sin \frac{1}{2} n\pi + 0 - 0 \right)$$

$$= -\frac{8}{n\pi} \cos \frac{1}{2} n\pi + \frac{16}{n^2\pi} \sin \frac{1}{2} n\pi \quad \text{--- (1)}$$

$$\begin{aligned} u &= x \\ du &= 1 \\ dv &= \sin \frac{n\pi x}{8} \\ v &= -\frac{\cos \frac{n\pi x}{8}}{\frac{n\pi}{8}} \end{aligned}$$

$$\textcircled{1} + \textcircled{11}$$

So,

$$f(n) = \sum_{n=1}^{\infty} \frac{32}{n^2} \sin \frac{n\pi}{2} \sin \frac{n\pi}{8} \quad (\text{Ans})$$

$$f(x) = \frac{a_0}{2} + \sum_{n=1}^{\infty} a_n \cos nx + \sum_{n=1}^{\infty} b_n \sin nx$$

$$\Rightarrow \frac{1}{\pi} \left[-\int_{-\pi}^0 x \sin(nx) dx + \int_0^{\pi} x \sin(nx) dx \right]$$

$$\Rightarrow \frac{1}{\pi} \left[-(0-0) + C \left(\frac{\pi(0-0)}{n} \right)^n + 0 - \frac{\pi(0-0)^n}{n} + 0 + 0 - 0 \right]$$

$$b_n \Rightarrow 0$$

$$b_n = 0$$

$$a_n = \frac{1}{\pi} \int_{-\pi}^{\pi} |x| \cos(nx) dx$$

$$\Rightarrow \frac{1}{\pi} \left[\int_{-\pi}^0 (-x) \cos nx dx + \int_0^{\pi} x \cos nx dx \right]$$

$$\Rightarrow \frac{1}{\pi} \left[- \int_{-\pi}^0 x \cos nx dx + \int_0^{\pi} x \cos nx dx \right]$$

$$\int x \cos nx$$

$u = x$
 $du = 1$
 $dv = \cos nx$
 $v = \frac{\sin nx}{n}$

$$= \frac{x \sin nx}{n} - \int \frac{\sin nx}{n}$$

$$= \frac{x \sin nx}{n} + \frac{\cos nx}{n^2}$$

$$\Rightarrow \frac{1}{\pi} \left[- \left[\frac{x \sin nx}{n} + \frac{\cos nx}{n^2} \right]_{-\pi}^0 + \left[\frac{x \sin nx}{n} + \frac{\cos nx}{n^2} \right]_0^{\pi} \right]$$

$$\Rightarrow \frac{1}{\pi} \left[- \left(0 + \frac{1}{n^2} - 0 - \frac{(-1)^n}{n^2} \right) + 0 + \frac{(-1)^n}{n^2} - 0 - \frac{1}{n^2} \right]$$

$$\Rightarrow \frac{1}{\pi} \left[-\frac{1}{n^2} + \frac{(-1)^n}{n^2} + \frac{(-1)^n}{n^2} - \frac{1}{n^2} \right]$$

$$a_n = \frac{1}{\pi} \left[\frac{2(-1)^n - 2}{n^2} \right] = \frac{2}{\pi} \frac{(-1)^n - 1}{n^2}$$

$$a_0 = \frac{2}{\pi} \frac{(-1)^0 - 1}{0^2} = \frac{1}{\pi} \int_{-\pi}^{\pi} |x| dx$$

$$= \frac{1}{\pi} \left[\int_{-\pi}^0 (-x) dx + \int_0^{\pi} x dx \right]$$

$$= \frac{1}{\pi} \left[\left[-\frac{x^2}{2} \right]_{-\pi}^0 + \left[\frac{x^2}{2} \right]_0^{\pi} \right]$$

$$= \frac{1}{\pi} \left(-\frac{0}{2} + \frac{\pi^2}{2} + \frac{\pi^2}{2} - 0 \right)$$

$$a_0 = \frac{\pi}{2}$$

$$|x| = \frac{\pi}{2} - \sum_{n=1}^{\infty} \frac{2}{\pi} \frac{(-1)^n - 1}{n^2} \cos nx$$

$$= \frac{\pi}{2} - \frac{2}{\pi} \sum_{n=1}^{\infty} \frac{(-1)^n - 1}{n^2} (-1)^n$$

$$= \frac{\pi}{2} - \frac{2}{\pi} \sum_{n=1}^{\infty} \frac{(-1)^n ((-1)^n - 1)}{n^2}$$

$$= \frac{\pi}{2} - \frac{2}{\pi} \sum_{n=1}^{\infty} \frac{(-1)^{n+1} - (-1)^n}{n^2}$$

$$\frac{1}{\pi} \int_{-\pi}^{\pi} [f(x)]^2 dx = \frac{a_0^2}{2} + \sum_{n=1}^{\infty} (a_n^2 + b_n^2)$$

$$\frac{1}{\pi} \int_{-\pi}^{\pi} |x|^2 dx$$

$$\begin{aligned} &= \frac{1}{\pi} \left[\int_0^{\pi} x^2 dx + \int_{-\pi}^0 (-x)^2 dx \right] \\ &= \frac{1}{\pi} \left[\left[\frac{x^3}{3} \right]_0^{\pi} + \left[\frac{x^3}{3} \right]_{-\pi}^0 \right] \\ &= \frac{1}{\pi} \left(\frac{\pi^3}{3} + \frac{\pi^3}{3} \right) \\ &= \frac{2\pi^2}{3} \end{aligned}$$

$$\frac{a_0^2}{2} + \sum_{n=1}^{\infty} (a_n^2 + b_n^2)$$

$$\frac{\pi^2}{2} + \sum_{n=1}^{\infty} \left[\frac{2}{\pi} \frac{(-1)^n - 1}{n^2} \right]^2 + 0$$

$$\frac{\pi^2}{2} + \sum_{n=1}^{\infty} \underbrace{\frac{4}{\pi^2 n^4} (-1)^n - 1}_{\downarrow}$$

when n is even

$$\frac{4}{\pi^2 n^4} (1 - 1)^2 = 0$$

when n is odd

$$\frac{4}{\pi^2 n^4} (-2)^2 = \frac{16}{\pi^2 n^4}$$

$$\frac{\pi^2}{2} + \frac{16}{\pi^2 (1)^4} + \frac{16}{\pi^2 (3)^4} + \dots$$

$$\frac{\pi^2}{2} + \frac{16}{\pi^2} \left(\frac{1}{1^4} + \frac{1}{3^4} + \frac{1}{5^4} + \dots \right)$$

So final eqn

$$\frac{2}{3} \pi^2 = \frac{\pi^2}{2} + \frac{16}{\pi^2} \left(1 + \frac{1}{3^4} + \frac{1}{5^4} + \dots \right)$$

$$\frac{\pi^2}{6} = \frac{16}{\pi^2} \left(1 + \frac{1}{3^4} + \frac{1}{5^4} + \dots \right)$$

$$\frac{\pi^4}{96} = 1 + \frac{1}{3^4} + \frac{1}{5^4} + \dots$$

$$\therefore 1 + \frac{1}{3^4} + \frac{1}{5^4} + \dots = \frac{\pi^4}{96} \quad (Ans)$$